cparser/Unblock.ml
@@ -154,6 +154,7 @@ let rec expand_expr islocal env e =
 (* Elimination of compound literals within an initializer. *)
 
 and expand_init islocal env i =
+
   let rec expand i =
     match i with
     (* The following "flattening" is not C99.  GCC documents it; whether
@@ -169,7 +170,7 @@ and expand_init islocal env i =
     | Init_single e ->
         Init_single (expand_expr islocal env e)
     | Init_array il ->
-        Init_array (List.map expand il)
+        Init_array (List.rev (List.rev_map expand il))
     | Init_struct(id, flds) ->
         Init_struct(id, List.map (fun (f, i) -> (f, expand i)) flds)
     | Init_union(id, fld, i) ->
